Add transition typeclass with serial witness

Ctl/Definition.v
@@ -1,14 +1,24 @@
 Require Import Ctl.Paths.
 Require Import BinaryRelations.
+Require Import Isomorphisms.
 
+Class transition {A} (R: relation A) := 
+  {trans_serial: serial_witness R}.
 
-Definition tprop state := relation state -> state -> Prop.
+(* Definition tprop state := relation state -> state -> Prop. *)
+
+Definition tprop state :=
+  forall R: relation state,
+    transition R ->
+    state ->
+    Prop.
 
 Delimit Scope tprop_scope with tprop.
 Open Scope tprop_scope.
 
-Definition tentails {state} (R: relation state) (s: state) (P: tprop state) :=
-  P R s.
+Definition tentails {state} (R: relation state) {t: transition R}
+  (s: state) (P: tprop state) :=
+  P R t s.
 Notation "R @ s ⊨ P" := (tentails R s P)   (at level 70, format "R  @ s  ⊨  P") : tprop_scope.
 Notation "R @ s ⊭ P" := (~ tentails R s P) (at level 70, format "R  @ s  ⊭  P") : tprop_scope.
 
@@ -16,28 +26,28 @@ Notation "R @ s ⊭ P" := (~ tentails R s P) (at level 70, format "R  @ s  ⊭  
 (* State props *)
 
 Definition ttop {state}: tprop state :=
-  fun _ _ => True.
+  fun _ _ _ => True.
 
 Definition tbot {state}: tprop state :=
-  fun _ _ => False.
+  fun _ _ _ => False.
 
 Definition tconj {state} (P Q: tprop state): tprop state :=
-  fun R s => R @s ⊨ P /\ R @s ⊨ Q.
+  fun R _ s => R @s ⊨ P /\ R @s ⊨ Q.
 
 Definition tdisj {state} (P Q: tprop state): tprop state := 
-  fun R s => R @s ⊨ P \/ R @s ⊨ Q.
+  fun R _ s => R @s ⊨ P \/ R @s ⊨ Q.
 
 Definition timpl {state} (P Q: tprop state): tprop state :=
-  fun R s => R @s ⊨ P -> R @s ⊨ Q.
+  fun R _ s => R @s ⊨ P -> R @s ⊨ Q.
 
 Definition tbiimpl {state} (P Q: tprop state): tprop state :=
-  fun R s => R @s ⊨ P <-> R @s ⊨ Q.
+  fun R _ s => R @s ⊨ P <-> R @s ⊨ Q.
 
 Definition tnot {state} (P: tprop state): tprop state :=
-  fun R s => R @s ⊭ P.
+  fun R _ s => R @s ⊭ P.
 
 Definition tlift {state} (P: state -> Prop): tprop state :=
-  fun _ s => P s.
+  fun _ _ s => P s.
 
 (* State prop notations *)
 Notation "⊤"      := (ttop) : tprop_scope.
@@ -47,38 +57,37 @@ Notation "P ∨ Q"  := (tdisj P Q)   (at level 55, right associativity) : tprop_
 Notation "P ⟶ Q" := (timpl P Q)   (at level 68,  right associativity) : tprop_scope.
 Notation "P ⟷ Q" := (tbiimpl P Q) (at level 65,  right associativity) : tprop_scope.
 Notation "¬ P"    := (tnot P)      (at level 40, format "¬ P") : tprop_scope.
-(* Notation "¬ P"    := (tnot P)      (at level 69, format "¬ P") : tprop_scope. *)
 Notation "⟨ P ⟩"   := (tlift P)     (format "⟨ P ⟩"): tprop_scope.
 
 
 (* path-quantifying props *)
 
 Definition AX {state} (P: tprop state) : tprop state :=
-  fun R s => forall s', R s s' -> R @s' ⊨ P.
+  fun R t s => forall s', R s s' -> R @s' ⊨ P.
   
 Definition EX {state} (P: tprop state) : tprop state :=
-  fun R s => exists s', R s s' /\ R @s' ⊨ P.
+  fun R t s => exists s', R s s' /\ R @s' ⊨ P.
 
 Definition AG {state} (P: tprop state) : tprop state :=
-  fun R s => forall (p: path R s) s', in_path s' p -> R @s' ⊨ P.
+  fun R t s => forall (p: path R s) s', in_path s' p -> R @s' ⊨ P.
 
 Definition EG {state} (P: tprop state) : tprop state :=
-  fun R s => exists p: path R s, forall s', in_path s' p -> R @s' ⊨ P.
+  fun R t s => exists p: path R s, forall s', in_path s' p -> R @s' ⊨ P.
 
 Definition AF {state} (P: tprop state) : tprop state :=
-  fun R s => forall p: path R s, exists s', in_path s' p /\ R @s' ⊨ P.
+  fun R t s => forall p: path R s, exists s', in_path s' p /\ R @s' ⊨ P.
   
 Definition EF {state} (P: tprop state) : tprop state :=
-  fun R s => exists (p: path R s) s', in_path s' p /\ R @s' ⊨ P.
+  fun R t s => exists (p: path R s) s', in_path s' p /\ R @s' ⊨ P.
 
 Definition AU {state} (P Q: tprop state) : tprop state :=
-  fun R s => forall p: path R s, exists sQ i,
+  fun R t s => forall p: path R s, exists sQ i,
     in_path_at sQ i p /\ 
     (forall sP, in_path_before sP i p -> R @sP ⊨ P) /\ 
     R @sQ ⊨ Q.
 
 Definition EU {state} (P Q: tprop state) : tprop state :=
-  fun R s => exists (p: path R s) sQ i,
+  fun R t s => exists (p: path R s) sQ i,
     in_path_at sQ i p /\ 
     (forall sP, in_path_before sP i p -> R @sP ⊨ P) /\ 
     R @sQ ⊨ Q.
@@ -88,7 +97,7 @@ Notation "A[ P 'U' Q ]" := (AU P Q) (at level 40, format "A[ P  'U'  Q ]") : tpr
 Notation "E[ P 'U' Q ]" := (EU P Q) (at level 40, format "E[ P  'U'  Q ]") : tprop_scope.
 
 Definition AW {state} (P Q: tprop state) : tprop state :=
-  fun R s => R @s ⊨ A[P U Q] ∨ ¬AF P.
+  fun R t s => R @s ⊨ A[P U Q] ∨ ¬AF P.
   (* fun R s => forall s' (seq: R#* s s'),
     (forall x, in_seq x seq -> R @x ⊨ P ∧ ¬Q) ->
     forall s'', 
